Added putchar proofs

progs/io_combine.v
@@ -22,10 +22,12 @@ Notation "' p <- t1 ;; t2" :=
 (at level 100, t1 at next level, p pattern, right associativity) : itree_scope.
 Require Import ITree.Interp.Traces.
 Require Import Ensembles.
+Require Import VST.progs.io_specs.
 Require Import VST.progs.io_dry.
 Require Import VST.progs.io_os_specs.
 Require Import VST.progs.io_os_connection.
 Require Import VST.progs.os_combine.
+Require Import VST.progs.dry_mem_lemmas.
 
 Section IO_safety.
 
@@ -36,22 +38,22 @@ Definition ext_link := ext_link_prog prog.
 
 Definition sys_getc_wrap_spec (abd : RData) : option (RData * val * trace) :=
   match sys_getc_spec abd with
-  | Some abd' => Some (abd', get_sys_ret abd', trace_of_ostrace (strip_common_prefix IOEvent_eq abd.(io_log) abd'.(io_log)))
+  | Some abd' => Some (abd', get_sys_ret abd', trace_of_ostrace (strip_common_prefix IOEvent_eq abd.(io_rx_log) abd'.(io_rx_log)))
   | None => None
   end.
 
 Definition sys_putc_wrap_spec (cv : val) (abd : RData) : option (RData * val * trace) :=
-(*  (* Make sure argument is set *)
+  (* Make sure argument is set *)
   match cv, get_sys_arg1 abd with
   | Vint c, Vint c' =>
-    if eq_dec.eq_dec c c' then*)
+    if eq_dec.eq_dec c c' then
       match sys_putc_spec abd with
-      | Some abd' => Some (abd', get_sys_ret abd', trace_of_ostrace (strip_common_prefix IOEvent_eq abd.(io_log) abd'.(io_log)))
+      | Some abd' => Some (abd', get_sys_ret abd', trace_of_ostrace (strip_common_prefix IOEvent_eq abd.(io_tx_log) abd'.(io_tx_log)))
       | None => None
       end
-(*    else None
+    else None
   | _, _ => None
-  end*).
+  end.
 
 Definition IO_ext_sem e (args : list val) s :=
   if oi_eq_dec (Some (ext_link "putchar"%string, funsig2signature ([(1%positive, tint)], tint) cc_default))
@@ -75,7 +77,7 @@ Variable (R_mem : block -> Z).
 
 (* Because putchar and getchar don't use memory, these functions don't either. *)
 Definition IO_inj_mem (e : external_function) (args : list val) (m : mem) t s :=
-  valid_trace s /\ t = trace_of_ostrace s.(io_log).
+  valid_trace s /\ t = trace_of_ostrace s.(io_rx_log).
 Definition OS_mem (e : external_function) (args : list val) m (s : RData) : mem := m.
 (* In general, this could look like:
   if oi_eq_dec (Some (ext_link "putchars"%string, ...) (ef_id_sig ext_link e) then
@@ -85,7 +87,7 @@ Definition OS_mem (e : external_function) (args : list val) m (s : RData) : mem 
   else ...
 *)
 
-Instance IO_Espec : OracleKind := io_specs.IO_Espec ext_link.
+Instance IO_Espec : OracleKind := IO_Espec ext_link.
 
 Theorem IO_OS_soundness:
  forall {CS: compspecs} (initial_oracle: OK_ty) V G m,
@@ -106,19 +108,16 @@ Proof.
       destruct H1 as (? & ? & Hpre); subst.
       destruct s; simpl in *.
       unfold sys_putc_wrap_spec in *.
-(*      destruct get_sys_arg1 eqn:Harg; try discriminate.
-      destruct (eq_dec _ _); subst; try discriminate.*)
+      destruct get_sys_arg1 eqn:Harg; try discriminate.
+      destruct (eq_dec _ _); subst; try discriminate.
       destruct sys_putc_spec eqn:Hspec; inv H3.
-(*      eapply sys_putc_correct in Hspec as (? & -> & [? Hpost ?]); eauto.
-      split.
-      { admit. (* waiting for valid trace condition *) }
-      eauto.*) admit. (* waiting for putc proof *)
+      eapply sys_putc_correct in Hspec as (? & -> & [? Hpost ?]); eauto.
     + destruct w as (? & _ & ?).
       destruct H1 as (? & ? & Hpre); subst.
       destruct s; simpl in *.
       unfold sys_getc_wrap_spec in *.
       destruct (sys_getc_spec) eqn:Hspec; inv H3.
-      eapply sys_getc_correct in Hspec as (? & -> & [? Hpost ? ?]); eauto.
+      eapply sys_getc_correct with (m1 := m) in Hspec as (? & -> & [? Hpost ? ?]); eauto.
       * split; auto; do 2 eexists; eauto.
         unfold getchar_post, getchar_post' in *.
         destruct Hpost as [? Hpost]; split; auto.
@@ -129,12 +128,165 @@ Proof.
         apply Traces.sutt_trace_incl; auto.
   - apply juicy_dry_specs.
   - apply dry_spec_mem.
-Admitted.
+Qed.
 
 (* relate to OS's external events *)
   Notation ge := (globalenv prog).
 
-  Inductive OS_safeN_trace : nat -> @trace io_specs.IO_event unit -> Ensemble (@trace io_specs.IO_event unit * RData) -> OK_ty -> RData -> corestate -> mem -> Prop :=
+(* for now, this is only proved for getchar *)
+Definition IO_ext_sem' e (args : list val) s :=
+  if oi_eq_dec  (Some (ext_link "getchar"%string, funsig2signature ([], tint) cc_default))
+    (ef_id_sig ext_link e) then
+    match sys_getc_wrap_spec s with
+    | Some (s', ret, t') => Some (s', Some ret, t')
+    | None => None
+    end
+  else Some (s, None, TEnd).
+
+Definition IO_specs' (ext_link : string -> ident) :=
+  [(ext_link "getchar"%string, getchar_spec)].
+
+Instance IO_Espec' : OracleKind := add_funspecs IO_void_Espec ext_link (IO_specs' ext_link).
+
+Definition io_ext_spec := OK_spec.
+
+Program Definition io_dry_spec : external_specification mem external_function IO_itree.
+Proof.
+  unshelve econstructor.
+  - intro e.
+    pose (ext_spec_type io_ext_spec e) as T; simpl in T.
+    destruct (oi_eq_dec _ _); [|exact False];
+      match goal with T := (_ * ?A)%type |- _ => exact (mem * A)%type end.
+  - simpl; intros.
+    destruct (oi_eq_dec _ _); [|contradiction].
+    + destruct X as (m0 & _ & w).
+      exact (X1 = [] /\ m0 = X3 /\ getchar_pre X3 w X2).
+  - simpl; intros.
+    destruct (oi_eq_dec _ _); [|contradiction].
+    + destruct X as (m0 & _ & w).
+      destruct X1; [|exact False].
+      destruct v; [exact False | | exact False | exact False | exact False | exact False].
+      exact (getchar_post m0 X3 i w X2).
+  - intros; exact False.
+Defined.
+
+Definition dessicate : forall ef (jm : juicy_mem), ext_spec_type io_ext_spec ef -> ext_spec_type io_dry_spec ef.
+Proof.
+  simpl; intros.
+  destruct (oi_eq_dec _ _); [|assumption].
+  destruct X as [_ X]; exact (m_dry jm, X).
+Defined.
+
+Theorem juicy_dry_specs : juicy_dry_ext_spec _ io_ext_spec io_dry_spec dessicate.
+Proof.
+  split; [|split]; try reflexivity; simpl.
+  - unfold funspec2pre, dessicate; simpl.
+    intros ?; if_tac; [|contradiction].
+    + unfold funspec2pre; simpl.
+      intros; subst.
+      destruct t as (? & ? & k); simpl in *.
+      destruct H1 as (? & phi0 & phi1 & J & Hpre & Hr & Hext).
+      destruct e; inv H; simpl in *.
+      destruct vl; try contradiction.
+      unfold putchar_pre; split; auto; split; auto.
+      unfold SEPx in Hpre; simpl in Hpre.
+      rewrite seplog.sepcon_emp in Hpre.
+      destruct Hpre as (_ & _ & ? & ? & Htrace).
+      apply has_ext_eq in Htrace.
+      eapply join_sub_joins_trans in Hext; [|eexists; apply ghost_of_join; eauto].
+      unfold getchar_pre.
+      eapply has_ext_join in Hext as []; [| rewrite Htrace; reflexivity | apply join_comm, core_unit]; subst; auto.
+  - unfold funspec2pre, funspec2post, dessicate; simpl.
+    intros ?; if_tac; [|contradiction].
+    + unfold funspec2pre, funspec2post, dessicate; simpl.
+      intros; subst.
+      destruct H0 as (_ & vl & z0 & ? & _ & phi0 & phi1' & J & Hpre & ? & ?).
+      destruct t as (phi1 & t); subst; simpl in *.
+      destruct t as (? & k); simpl in *.
+      unfold SEPx in Hpre; simpl in Hpre.
+      rewrite seplog.sepcon_emp in Hpre.
+      destruct Hpre as (_ & _ & ? & ? & Htrace).
+      pose proof (has_ext_eq _ _ Htrace) as Hgx.
+      destruct v; try contradiction.
+      destruct v; try contradiction.
+      destruct H4 as (Hmem & ? & Hw); simpl in Hw; subst.
+      rewrite <- Hmem in *.
+      rewrite rebuild_same in H2.
+      unshelve eexists (age_to.age_to (level jm) (set_ghost phi0 [Some (ext_ghost x, NoneP)] _)), (age_to.age_to (level jm) phi1'); auto.
+      split; [|split3].
+      * eapply age_rejoin; eauto.
+        intro; rewrite H2; auto.
+      * exists i.
+        split3; simpl.
+        -- split; auto.
+        -- split; auto; split; unfold liftx; simpl; unfold lift.lift; auto; discriminate.
+        -- unfold SEPx; simpl.
+             rewrite seplog.sepcon_emp.
+             unfold ITREE; exists x; split; [if_tac; auto|].
+             { subst; apply eutt_sutt, UpToTausCore.Reflexive_eutt. }
+             eapply age_to.age_to_pred, change_has_ext; eauto.
+      * eapply necR_trans; eauto; apply age_to.age_to_necR.
+      * rewrite H3; eexists; constructor; constructor.
+        instantiate (1 := (_, _)).
+        constructor; simpl; [|constructor; auto].
+        apply ext_ref_join.
+Qed.
+
+Instance mem_evolve_refl : Reflexive mem_evolve.
+Proof.
+  repeat intro.
+  destruct (access_at x loc Cur); auto.
+  destruct p; auto.
+Qed.
+
+Lemma dry_spec_mem : ext_spec_mem_evolve _ io_dry_spec.
+Proof.
+  intros ??????????? Hpre Hpost.
+  simpl in Hpre, Hpost.
+  simpl in *.
+  if_tac in Hpre; [|contradiction].
+  - destruct w as (m0 & _ & w).
+    destruct Hpre as (_ & ? & Hpre); subst.
+    destruct v; try contradiction.
+    destruct v; try contradiction.
+    destruct Hpost; subst.
+    reflexivity.
+Qed.
+
+Theorem IO_OS_soundness':
+ forall {CS: compspecs} (initial_oracle: OK_ty) V G m,
+   semax_prog_ext prog initial_oracle V G ->
+   Genv.init_mem prog = Some m ->
+   exists b, exists q, exists m',
+     Genv.find_symbol (Genv.globalenv prog) (prog_main prog) = Some b /\
+     initial_core (cl_core_sem (globalenv prog))
+         0 m q m' (Vptr b Ptrofs.zero) nil /\
+   forall n, exists traces, ext_safeN_trace(J := OK_spec) prog IO_ext_sem' IO_inj_mem OS_mem valid_trace n TEnd traces initial_oracle q m' /\
+     forall t, In _ traces t -> exists z', consume_trace initial_oracle z' t.
+Proof.
+  intros; eapply OS_soundness with (dryspec := io_dry_spec); eauto.
+  - unfold IO_ext_sem'; intros; simpl in *.
+    destruct H2 as [Hvalid Htrace].
+    if_tac; [|contradiction].
+    + destruct w as (? & _ & ?).
+      destruct H1 as (? & ? & Hpre); subst.
+      destruct s; simpl in *.
+      unfold sys_getc_wrap_spec in *.
+      destruct (sys_getc_spec) eqn:Hspec; inv H3.
+      eapply sys_getc_correct with (m1 := m) in Hspec as (? & -> & [? Hpost ? ?]); eauto.
+      * split; auto; do 2 eexists; eauto.
+        unfold getchar_post, getchar_post' in *.
+        destruct Hpost as [? Hpost]; split; auto.
+        destruct Hpost as [[]|[-> ->]]; split; try (simpl in *; omega).
+        -- rewrite if_false by omega; eauto.
+        -- rewrite if_true; auto.
+      * unfold getchar_pre, getchar_pre' in *.
+        apply Traces.sutt_trace_incl; auto.
+  - apply juicy_dry_specs.
+  - apply dry_spec_mem.
+Qed.
+
+  Inductive OS_safeN_trace : nat -> @trace io_events.IO_event unit -> Ensemble (@trace io_events.IO_event unit * RData) -> OK_ty -> RData -> corestate -> mem -> Prop :=
   | OS_safeN_trace_0: forall t z s c m, OS_safeN_trace O t (Singleton _ (TEnd, s)) z s c m
   | OS_safeN_trace_step:
       forall n t traces z s c m c' m',
@@ -148,7 +300,7 @@ Admitted.
          (Hargsty : Val.has_type_list args (sig_args (ef_sig e)))
          (Hretty : step_lemmas.has_opttyp ret (sig_res (ef_sig e))),
          IO_inj_mem e args m t s ->
-         IO_ext_sem e args s = Some (s', ret, t') ->
+         IO_ext_sem' e args s = Some (s', ret, t') ->
          m' = OS_mem e args m s' ->
          (n' <= n)%nat ->
          valid_trace s' /\ exists traces' z' c', consume_trace z z' t' /\
@@ -158,7 +310,7 @@ Admitted.
       (forall t1, In _ traces t1 ->
         exists s s' ret m' t' n', Val.has_type_list args (sig_args (ef_sig e)) /\
          step_lemmas.has_opttyp ret (sig_res (ef_sig e)) /\
-         IO_inj_mem e args m t s /\ IO_ext_sem e args s = Some (s', ret, t') /\ m' = OS_mem e args m s' /\
+         IO_inj_mem e args m t s /\ IO_ext_sem' e args s = Some (s', ret, t') /\ m' = OS_mem e args m s' /\
          (n' <= n)%nat /\ valid_trace s' /\ exists traces' z' c', consume_trace z z' t' /\
            cl_after_external ret c = Some c' /\ OS_safeN_trace n' (app_trace t t') traces' z' s' c' m' /\
         exists t'' sf, In _ traces' (t'', sf) /\ t1 = (app_trace t' t'', sf)) ->
@@ -180,20 +332,13 @@ Local Ltac destruct_spec Hspec :=
   | match ?x with _ => _ end = _ => destruct x eqn:?; subst; inj; try discriminate
   end.
 
-  Lemma IO_ext_sem_trace : forall e args s s' ret t, valid_trace s -> IO_ext_sem e args s = Some (s', ret, t) ->
-    s.(io_log) = common_prefix IOEvent_eq s.(io_log) s'.(io_log) /\
-    t = trace_of_ostrace (strip_common_prefix IOEvent_eq s.(io_log) s'.(io_log)).
+  Lemma IO_ext_sem_trace : forall e args s s' ret t, valid_trace s -> IO_ext_sem' e args s = Some (s', ret, t) ->
+    s.(io_rx_log) = common_prefix IOEvent_eq s.(io_rx_log) s'.(io_rx_log) /\
+    t = trace_of_ostrace (strip_common_prefix IOEvent_eq s.(io_rx_log) s'.(io_rx_log)).
   Proof.
     intros until 1.
-    unfold IO_ext_sem.
-    if_tac; [|if_tac].
-    - unfold sys_putc_wrap_spec.
-      destruct args as [| (*[]*)? [|]]; try discriminate.
-      (*destruct get_sys_arg1 eqn: Harg; try discriminate.
-      destruct (eq_dec _ _); try discriminate.*)
-      destruct sys_putc_spec eqn: Hputc; inversion 1; subst; split; auto.
-      (* TODO: Fix rx vs tx log *)
-      admit. (* waiting for putc proof *)
+    unfold IO_ext_sem'.
+    if_tac.
     - unfold sys_getc_wrap_spec.
       destruct sys_getc_spec eqn: Hgetc; inversion 1; subst; split; auto.
       pose proof Hgetc as Hspec.
@@ -206,7 +351,7 @@ Local Ltac destruct_spec Hspec :=
       repeat (rewrite ZMap.gss in * || rewrite ZMap.gso in * by easy); subst; inj; reflexivity.
     - inversion 1.
       rewrite common_prefix_full, strip_all; auto.
-  Admitted.
+  Qed.
 
   Lemma app_trace_end : forall t, app_trace (trace_of_ostrace t) TEnd = trace_of_ostrace t.
   Proof.
@@ -224,9 +369,9 @@ Local Ltac destruct_spec Hspec :=
   Qed.
 
   Lemma OS_trace_correct' : forall n t traces z s0 c m
-    (Hvalid : valid_trace s0) (Ht : t = trace_of_ostrace s0.(io_log)),
+    (Hvalid : valid_trace s0) (Ht : t = trace_of_ostrace s0.(io_rx_log)),
     OS_safeN_trace n t traces z s0 c m ->
-    forall t' sf, In _ traces (t', sf) -> valid_trace sf /\ app_trace (trace_of_ostrace s0.(io_log)) t' = trace_of_ostrace sf.(io_log).
+    forall t' sf, In _ traces (t', sf) -> valid_trace sf /\ app_trace (trace_of_ostrace s0.(io_rx_log)) t' = trace_of_ostrace sf.(io_rx_log).
   Proof.
     induction n as [n IHn] using lt_wf_ind; intros; inv H.
     - inv H0.
@@ -242,7 +387,7 @@ Local Ltac destruct_spec Hspec :=
       { rewrite Htrace, app_trace_strip; auto. }
   Qed.
 
-  Lemma init_log_valid : forall s, io_log s = [] -> console s = {| cons_buf := []; rpos := 0 |} -> valid_trace s.
+  Lemma init_log_valid : forall s, io_rx_log s = [] -> console s = {| cons_buf := []; rpos := 0 |} -> valid_trace s.
   Proof.
     intros s Hinit Hcon.
     constructor; rewrite Hinit; repeat intro; try (pose proof app_cons_not_nil; congruence).
@@ -252,9 +397,9 @@ Local Ltac destruct_spec Hspec :=
   Qed.
 
   Lemma OS_trace_correct : forall n traces z s0 c m
-    (Hinit : s0.(io_log) = []) (Hcon : s0.(console) = {| cons_buf := []; rpos := 0 |}),
+    (Hinit : s0.(io_rx_log) = []) (Hcon : s0.(console) = {| cons_buf := []; rpos := 0 |}),
     OS_safeN_trace n TEnd traces z s0 c m ->
-    forall t sf, In _ traces (t, sf) -> valid_trace sf /\ t = trace_of_ostrace sf.(io_log).
+    forall t sf, In _ traces (t, sf) -> valid_trace sf /\ t = trace_of_ostrace sf.(io_rx_log).
   Proof.
     intros; eapply OS_trace_correct' in H as [? Htrace]; eauto.
     split; auto.
@@ -288,7 +433,7 @@ Local Ltac destruct_spec Hspec :=
   Qed.
 
   Lemma ext_safe_OS_safe : forall n t traces z q m s0 (Hvalid : valid_trace s0),
-    ext_safeN_trace(J := OK_spec) prog IO_ext_sem IO_inj_mem OS_mem valid_trace n t traces z q m ->
+    ext_safeN_trace(J := OK_spec) prog IO_ext_sem' IO_inj_mem OS_mem valid_trace n t traces z q m ->
     exists traces', OS_safeN_trace n t traces' z s0 q m /\ forall t, In _ traces t <-> exists s, In _ traces' (t, s).
   Proof.
     induction n as [n IHn] using lt_wf_ind; intros; inv H.
@@ -301,7 +446,7 @@ Local Ltac destruct_spec Hspec :=
       eapply OS_safeN_trace_step; eauto.
     - exists (fun t1 => exists s s' ret m' t' n', Val.has_type_list args (sig_args (ef_sig e)) /\
          step_lemmas.has_opttyp ret (sig_res (ef_sig e)) /\
-         IO_inj_mem e args m t s /\ IO_ext_sem e args s = Some (s', ret, t') /\ m' = OS_mem e args m s' /\
+         IO_inj_mem e args m t s /\ IO_ext_sem' e args s = Some (s', ret, t') /\ m' = OS_mem e args m s' /\
          (n' <= n0)%nat /\ valid_trace s' /\ exists traces' z' c', consume_trace z z' t' /\
            cl_after_external ret q = Some c' /\ OS_safeN_trace n' (app_trace t t') traces' z' s' c' m' /\
         exists t'' sf, In _ traces' (t'', sf) /\ t1 = (app_trace t' t'', sf)); split.
@@ -330,12 +475,12 @@ Theorem IO_OS_ext:
      Genv.find_symbol (Genv.globalenv prog) (prog_main prog) = Some b /\
      initial_core (cl_core_sem (globalenv prog))
          0 m q m' (Vptr b Ptrofs.zero) nil /\
-   forall n s0, s0.(io_log) = [] -> s0.(console) = {| cons_buf := []; rpos := 0 |} ->
+   forall n s0, s0.(io_rx_log) = [] -> s0.(console) = {| cons_buf := []; rpos := 0 |} ->
     exists traces, OS_safeN_trace n TEnd traces initial_oracle s0 q m' /\
-     forall t s, In _ traces (t, s) -> exists z', consume_trace initial_oracle z' t /\ t = trace_of_ostrace s.(io_log) /\
-      valid_trace_user s.(io_log).
+     forall t s, In _ traces (t, s) -> exists z', consume_trace initial_oracle z' t /\ t = trace_of_ostrace s.(io_rx_log) /\
+      valid_trace_user s.(io_rx_log).
 Proof.
-  intros; eapply IO_OS_soundness in H as (? & ? & ? & ? & ? & Hsafe); eauto.
+  intros; eapply IO_OS_soundness' in H as (? & ? & ? & ? & ? & Hsafe); eauto.
   do 4 eexists; eauto; split; eauto; intros.
   destruct (Hsafe n) as (? & Hsafen & Htrace).
   eapply ext_safe_OS_safe in Hsafen as (? & Hsafen & Htrace').
